\begin{answer}

PROOF: according to the above results, 
\begin{eqnarray*}
\frac{p(y^{(i)} = 1\mid x^{(i)}) } {p(t^{(i)} = 1\mid x^{(i)})} 
    &=& p(y^{(i)} = 1 \mid t^{(i)} = 1) \\
    &=& \alpha \\
\end{eqnarray*}
This implies that:
\begin{eqnarray*}
h(x^{(i)}) 
    &\approx& p(y^{(i)} = 1\mid x^{(i)}) \\
    &\approx& \alpha p(t^{(i)} = 1\mid x^{(i)}) \\
    &\approx& \alpha
\end{eqnarray*}
The last step uses the assumption that $p(t^{(i)} = 1\mid x^{(i)})\approx 1$ when
$x^{(i)}\in V_{+}$.
\end{answer}
