\begin{answer}

The following derivatives w.r.t. $\eta$ is obvious:
\begin{eqnarray*}
\frac{\partial}{\partial \eta} p(y;\eta)
    &=& y b(y)\exp(\eta y -a(\eta)) - a'(\eta) b(y) \exp(\eta y - a(\eta)) \\
    &=& y p - a'(\eta) p \\
\end{eqnarray*}

The equation implies: 
\begin{eqnarray*}
    y p(y;\eta) =\frac{\partial}{\partial \eta} p(y;\eta) + a'(\eta) p(y;\eta) \\
\end{eqnarray*}

Sum over y gives the expectation of Y given X is:
\begin{eqnarray*}
\mathbb{E}(Y|X;\eta)
    &=& \int y p(y;\eta) dy \\
    &=& \frac{\partial}{\partial \eta}\int p(y;\eta)dy + a'(\eta)\int p(y;\eta)dy \\
    &=& a'(\eta)
\end{eqnarray*}
\end{answer}
