\begin{answer}

Again it is obvious that:

\begin{eqnarray*}
\frac{\partial^2}{\partial \eta^2} p(y;\eta)
    &=& y(y-a'(\eta)) b(y) \exp(\eta y-a(\eta))-b(y)a''(\eta)\exp(\eta y-a(\eta)) \\
    &-& a'(\eta)(y-a'(\eta))b(y)\exp(\eta y -a(\eta)) \\
    &=& ((y-a'(\eta))^2-a''(\eta))p
\end{eqnarray*}

Now consider the variance of Y:
\begin{eqnarray*}
\mathbb{V}(Y)
    &=& \mathbb{V}(Y-a'(\eta)) \\
    &=& \mathbb{E}(Y-a'(\eta))^2 - \mathbb{E}^2(Y-a'(\eta)) \\
    &=& \mathbb{E}(Y-a'(\eta))^2 \\
    &=& \int (y-a'(\eta))^2 p(y;\eta)dy \\
    &=& \frac{\partial^2}{\partial \eta^2} \int p(y;\eta)dy + a''(\eta) \int p(y;\eta)dy \\
    &=& a''(\eta)
\end{eqnarray*}
The second to third step holds because $\mathbb{E}(Y-a'(\eta)) = 0$ as proved in (a).

The 4th to 5th step is from the above derived $\frac{\partial^2}{\partial \eta^2} p(y;\eta)$ equation.

Q.E.D.

\end{answer}
